[WIP] Adding eq_name to Name

pcuic/theories/Name.v
@@ -1,28 +1,42 @@
 (* Distributed under the terms of the MIT license.   *)
 
-Require Import Coq.Strings.String.
-Require Import Coq.PArith.BinPos.
-Require Import List. Import ListNotations.
-From Template Require Import BasicAst.
+From Coq Require Import Ascii String Bool OrderedType Lia List Program Arith.
+Import ListNotations.
+From Template Require BasicAst.
+
+Module B := BasicAst.
 
 Class Name := {
   name : Set ;
   nNamed : string -> name ;
   nAnon : name ;
-  get_ident : name -> string
+  get_ident : name -> string ;
+  eq_name : name -> name -> bool ;
+  eq_name_spec : forall n1 n2, reflect (n1 = n2) (eq_name n1 n2)
 }.
 
-Definition basic_get_ident (n : BasicAst.name) : string :=
+Definition basic_get_ident (n : B.name) : string :=
   match n with
-  | BasicAst.nAnon => "XX"
-  | BasicAst.nNamed i => i
+  | B.nAnon => "XX"
+  | B.nNamed i => i
+  end.
+
+(* Problem of order, we would need ReflectEq and some instances already here
+   Anyway it should not be in ASTutils.
+ *)
+Definition basic_eq_name na nb :=
+  match na, nb with
+  | B.nAnon, B.nAnon => true
+  | B.nNamed a, B.nNamed b => eqb a b
+  | _, _ => false
   end.
 
 Local Instance BasicName : Name := {
   name := BasicAst.name ;
   nNamed := BasicAst.nNamed ;
   nAnon := BasicAst.nAnon ;
-  get_ident := basic_get_ident
+  get_ident := basic_get_ident ;
+  eq_name :=
 }.
 
 Local Instance Nameless : Name := {
